Remove references to δP in semantics and proofs
The existence and use of the `HasBool` class makes it unnecessary, and
it was always a little messy.

Strata/DL/Imperative/StmtSemantics.lean
@@ -23,64 +23,62 @@ evaluation relation `EvalCmd`.
 -/
 inductive EvalStmt (P : PureExpr) (Cmd : Type) (EvalCmd : EvalCmdParam P Cmd)
   [HasVarsImp P (List (Stmt P Cmd))] [HasVarsImp P Cmd] [HasFvar P] [HasVal P] [HasBool P] [HasBoolNeg P] :
-  SemanticEval P → SemanticEvalBool P → SemanticStore P → SemanticStore P →
+  SemanticEval P → SemanticStore P → SemanticStore P →
   Stmt P Cmd → SemanticStore P → Prop where
   | cmd_sem :
-    EvalCmd δ δP σ₀ σ c σ' →
+    EvalCmd δ σ₀ σ c σ' →
     -- We only require definedness on the statement level so that the requirement is fine-grained
     -- For example, if we require definedness on a block, then we won't be able to evaluate
     -- a block containing init x; havoc x, because it will require x to exist prior to the block
     isDefinedOver (HasVarsImp.modifiedVars) σ c →
     ----
-    EvalStmt P Cmd EvalCmd δ δP σ₀ σ (Stmt.cmd c) σ'
+    EvalStmt P Cmd EvalCmd δ σ₀ σ (Stmt.cmd c) σ'
 
   | block_sem :
-    EvalBlock P Cmd EvalCmd δ δP σ₀ σ b σ' →
+    EvalBlock P Cmd EvalCmd δ σ₀ σ b σ' →
     ----
-    EvalStmt P Cmd EvalCmd δ δP σ₀ σ (.block _ b) σ'
+    EvalStmt P Cmd EvalCmd δ σ₀ σ (.block _ b) σ'
 
   | ite_true_sem :
-    δP σ₀ σ c = .some true →
-    EvalBlock P Cmd EvalCmd δ δP σ₀ σ t σ' →
-    WellFormedSemanticEvalBool δ δP →
+    δ σ₀ σ c = .some HasBool.tt →
+    WellFormedSemanticEvalBool δ →
+    EvalBlock P Cmd EvalCmd δ σ₀ σ t σ' →
     ----
-    EvalStmt P Cmd EvalCmd δ δP σ₀ σ (.ite c t e) σ'
+    EvalStmt P Cmd EvalCmd δ σ₀ σ (.ite c t e) σ'
 
   | ite_false_sem :
-    δP σ₀ σ c = .some false →
-    EvalBlock P Cmd EvalCmd δ δP σ₀ σ e σ' →
-    WellFormedSemanticEvalBool δ δP →
+    δ σ₀ σ c = .some HasBool.ff →
+    WellFormedSemanticEvalBool δ →
+    EvalBlock P Cmd EvalCmd δ σ₀ σ e σ' →
     ----
-    EvalStmt P Cmd EvalCmd δ δP σ₀ σ (.ite c t e) σ'
+    EvalStmt P Cmd EvalCmd δ σ₀ σ (.ite c t e) σ'
 
   -- (TODO): Define semantics of `goto`.
 
 inductive EvalStmts (P : PureExpr) (Cmd : Type) (EvalCmd : EvalCmdParam P Cmd)
   [HasVarsImp P (List (Stmt P Cmd))] [HasVarsImp P Cmd] [HasFvar P] [HasVal P] [HasBool P] [HasBoolNeg P] :
-    SemanticEval P → SemanticEvalBool P →
-    SemanticStore P → SemanticStore P →
-  List (Stmt P Cmd) → SemanticStore P → Prop where
+    SemanticEval P → SemanticStore P → SemanticStore P →
+    List (Stmt P Cmd) → SemanticStore P → Prop where
   | stmts_none_sem :
-    EvalStmts P _ _ δ δP σ₀ σ [] σ
+    EvalStmts P _ _ δ σ₀ σ [] σ
   | stmts_some_sem :
-    EvalStmt P Cmd EvalCmd δ δP σ₀ σ s σ' →
-    EvalStmts P Cmd EvalCmd δ δP σ₀ σ' ss σ'' →
-    EvalStmts P Cmd EvalCmd δ δP σ₀ σ (s :: ss) σ''
+    EvalStmt P Cmd EvalCmd δ σ₀ σ s σ' →
+    EvalStmts P Cmd EvalCmd δ σ₀ σ' ss σ'' →
+    EvalStmts P Cmd EvalCmd δ σ₀ σ (s :: ss) σ''
 
 inductive EvalBlock (P : PureExpr) (Cmd : Type) (EvalCmd : EvalCmdParam P Cmd)
   [HasVarsImp P (List (Stmt P Cmd))] [HasVarsImp P Cmd] [HasFvar P] [HasVal P] [HasBool P] [HasBoolNeg P] :
-    SemanticEval P → SemanticEvalBool P →
-    SemanticStore P → SemanticStore P →
+    SemanticEval P → SemanticStore P → SemanticStore P →
   Block P Cmd → SemanticStore P → Prop where
   | block_sem :
-    EvalStmts P Cmd EvalCmd δ δP σ₀ σ b.ss σ' →
-    EvalBlock P Cmd EvalCmd δ δP σ₀ σ b σ'
+    EvalStmts P Cmd EvalCmd δ σ₀ σ b.ss σ' →
+    EvalBlock P Cmd EvalCmd δ σ₀ σ b σ'
 
 end
 
 theorem EvalCmdDefMonotone [HasFvar P] [HasBool P] [HasBoolNeg P] :
   isDefined σ v →
-  EvalCmd P δ δP σ₀ σ c σ' →
+  EvalCmd P δ σ₀ σ c σ' →
   isDefined σ' v := by
   intros Hdef Heval
   cases Heval <;> try exact Hdef
@@ -89,9 +87,9 @@ theorem EvalCmdDefMonotone [HasFvar P] [HasBool P] [HasBoolNeg P] :
   next _ _ Hup => exact UpdateStateDefMonotone Hdef Hup
 
 theorem EvalStmtsEmpty {P : PureExpr} {Cmd : Type} {EvalCmd : EvalCmdParam P Cmd}
-  { σ σ' σ₀: SemanticStore P } { δ : SemanticEval P } { δP: SemanticEvalBool P }
+  { σ σ' σ₀: SemanticStore P } { δ : SemanticEval P }
   [HasVarsImp P (List (Stmt P Cmd))] [HasVarsImp P Cmd] [HasFvar P] [HasVal P] [HasBool P] [HasBoolNeg P] :
-  EvalStmts P Cmd EvalCmd δ δP σ₀ σ ([]: (List (Stmt P Cmd))) σ' → σ = σ' := by
+  EvalStmts P Cmd EvalCmd δ σ₀ σ ([]: (List (Stmt P Cmd))) σ' → σ = σ' := by
   intros H; cases H <;> simp
 
 mutual
@@ -99,7 +97,7 @@ theorem EvalStmtDefMonotone
   [HasVal P] [HasFvar P] [HasBool P] [HasBoolVal P] [HasBoolNeg P]
   :
   isDefined σ v →
-  EvalStmt P (Cmd P) (EvalCmd P) δ δP σ₀ σ s σ' →
+  EvalStmt P (Cmd P) (EvalCmd P) δ σ₀ σ s σ' →
   isDefined σ' v := by
   intros Hdef Heval
   cases s
@@ -109,10 +107,10 @@ theorem EvalStmtDefMonotone
   next l b _ => cases Heval; next Hwf Hup => cases Hup; next Hup =>
     apply EvalStmtsDefMonotone (ss:=b.ss) <;> try assumption
   next c t b _ => cases Heval with
-  | ite_true_sem Hsome Heval =>
+  | ite_true_sem Hsome Hwf Heval =>
     cases Heval; next Heval =>
     apply EvalStmtsDefMonotone (ss:=t.ss) <;> try assumption
-  | ite_false_sem Hsome Heval =>
+  | ite_false_sem Hsome Hwf Heval =>
     cases Heval; next Heval =>
     apply EvalStmtsDefMonotone (ss:=b.ss) <;> try assumption
   case goto => cases Heval
@@ -124,7 +122,7 @@ theorem EvalStmtsDefMonotone
   [HasVal P] [HasFvar P] [HasBool P] [HasBoolVal P] [HasBoolNeg P]
   :
   isDefined σ v →
-  EvalStmts P (Cmd P) (EvalCmd P) δ δP σ₀ σ ss σ' →
+  EvalStmts P (Cmd P) (EvalCmd P) δ σ₀ σ ss σ' →
   isDefined σ' v := by
   intros Hdef Heval
   cases ss with
